src/Linearizable.v
@@ -5,8 +5,6 @@ Require Import EventCSL.
 Require Import FunctionalExtensionality.
 Import Morphisms.
 
-Set Universe Polymorphism.
-
 Section Linearizability.
 
   Variable A:Type.
