src/Linearizable2.v
@@ -6,8 +6,6 @@ Require Import FunctionalExtensionality.
 Require Import Automation.
 Import Morphisms.
 
-Set Universe Polymorphism.
-
 Section Linearizability.
 
   Variable A:Type.
