src/Pred.v
@@ -10,8 +10,6 @@ Require Import List.
 
 Set Implicit Arguments.
 
-Set Universe Polymorphism.
-
 
 (** ** Predicates *)
 
