src/PredCrash.v
@@ -7,8 +7,6 @@ Require Import Morphisms.
 
 Set Implicit Arguments.
 
-Set Universe Polymorphism.
-
 
 Notation "a |=> v" := (a |-> ((v, nil) : valuset))%pred (at level 35) : pred_scope.
 Notation "a |~> v" := (exists old, a |-> ((v, old) : valuset))%pred (at level 35) : pred_scope.
